Added the refinement procedure and lemmas in Composition.v

concur/Composition.v
@@ -118,6 +118,64 @@ Proof.
       constructor.
 Qed.
 
+Lemma move_wt_ext : cctrans (c_injp @ wt_c @ c_ext) (wt_c @ c_injp @ c_ext).
+Proof.
+  constructor.
+  econstructor. instantiate (1:= fun a b => fst a = fst (snd b) /\ snd (snd a) = snd (snd b)).
+  - red. intros. rename se2 into se3. rename q2 into q3.
+    simpl in w2. destruct w2 as [se1'1 [ [se1'2 sig] [se2 [w1 w2]]]].
+    destruct H as [Hsei [Hse1 Hse2]]. inv Hsei. inv H. rename se1'1 into se1.
+    destruct H0 as [q1' [Hqi [q2 [Hq1 Hq2]]]]. inv Hqi. rename q1' into q1.
+    exists (se2, (w1,(se2,((se2,sig) ,w2)))). intuition auto.
+    + constructor. auto. constructor. constructor. constructor. auto.
+    + inv Hq1. inv Hq2. inv H. simpl in *.
+      edestruct CallConv.has_type_inject_list as (vl2 & Hvl2 & Hvl & Hvl'); eauto.
+      exists (cq vf2 sg vl2 m2). split. constructor; eauto.
+      exists (cq vf2 sg vl2 m2). split. constructor; eauto.
+      constructor; eauto.
+      eapply CallConv.val_lessdef_inject_list_compose; eauto.
+    + destruct wp1' as [w1' [ss w2']]. destruct ss.
+      destruct H1 as [ACCE1 [_ ACCE2]]. simpl in ACCE1, ACCE2.
+      destruct wp1 as [wp1 [tt wp2aa]]. simpl in H4, H5. destruct wp2 as [tt1 [x y]]. simpl in H4, H5. subst x y.
+      rename wp2aa into wp2.
+      destruct H2 as [ACCI1 [_ ACCI2]]. simpl in ACCI1, ACCI2.
+      exists (tt, (w1', w2')). intuition auto.
+      repeat constructor; eauto.
+      repeat constructor; eauto. rename r2 into r3.
+      destruct H3 as [r2' [Hr1 [r2 [Hri Hr2]]]]. inv Hri.
+      repeat econstructor; eauto.
+      simpl. simpl in H0.
+      inv Hr1.
+      eapply val_has_type_inject; eauto.
+  - red. intros.  rename se2 into se3. rename q2 into q3.
+    simpl in wp1. destruct wp2 as [ss [x y]]. destruct ss.
+    destruct wp1 as [wp1 [ss wp2]]. destruct ss. inv H2.  simpl in H3, H4. subst x y.
+    destruct w1 as [se2' [w1 [se2 [[se2'' sig] w2]]]].
+    destruct H1 as [ACCI1 [X ACCI2]]. simpl in ACCI1, ACCI2. inv X.
+    destruct H as [Hse1 [Hsei Hse2]]. inv Hsei. inv H.
+    destruct H0 as [q2 [Hq1 [q2' [Hqi Hq2]]]]. inv Hqi. rename q2' into q2.
+    exists (se1,((se1,sig),(se2,(w1,w2)) )). intuition auto.
+    + repeat constructor; auto.
+    + repeat constructor; auto.
+    + exists q1. constructor.
+      inv Hq1. inv H. constructor. simpl in *. split; auto.
+      eapply val_has_type_list_inject; eauto.
+      exists q2. constructor; auto.
+    + destruct wp2' as [ss [wp1' wp2']]. destruct ss.
+      destruct H0 as [x [E1 E2]]. simpl in x,E1,E2. rename r2 into r3.
+      destruct H1 as [r1' [Hri [r2 [Hr1 Hr2]]]]. inv Hri.
+      exists (wp1', (tt, wp2')). intuition auto.
+      repeat constructor; auto.
+      inv Hr1. simpl in *.
+      exists (cr (Val.ensure_type vres2 (proj_sig_res sig)) m2').
+      split. constructor; eauto.
+      eapply CallConv.has_type_inject; eauto.
+      exists (cr (Val.ensure_type vres2 (proj_sig_res sig)) m2').
+      constructor. constructor. apply Val.ensure_has_type.
+      inv Hr2. econstructor; eauto.
+      eapply Val.inject_ensure_type_l; eauto.
+Qed.
+
 Inductive match_assoc_1 {A B C : Type}: (A * (B * C)) -> (A * B * C) -> Prop :=
 |match_assoc_1_intro a b c: match_assoc_1 (a,(b,c)) (a,b,c).
 
@@ -160,9 +218,6 @@ Proof.
     repeat econstructor; eauto.
     constructor.
 Qed.
-
-Lemma move_wt_ext : cctrans (c_injp @ wt_c @ c_ext) (wt_c @ c_injp @ c_ext).
-Admitted. (*should be the same as above*)
 
 Inductive match_assoc_2 {A B C : Type}: (A * B * C) -> (A * (B * C)) -> Prop :=
 |match_assoc_2_intro a b c: match_assoc_2 (a,b,c) (a,(b,c)).
@@ -210,3 +265,280 @@ Qed.
 
 
 
+(** Unification of the outgoing side *)
+
+Definition cc_compcert : GS.callconv li_c li_asm :=
+       ro @ wt_c @
+       cc_c_asm_injp_new.
+
+(** The C-level simulation convention *)
+Definition cc_c_level : GS.callconv li_c li_c := ro @ wt_c @ c_injp.
+
+Definition cc_compcert_1 : GS.callconv li_c li_asm :=
+    cc_c_level @
+    cc_c_locset @ cc_locset_mach @ cc_mach_asm.
+
+
+(** The first expand of cc_compcert for both directions *)
+Theorem cc_compcert_merge:
+  forall p tp,
+  GS.forward_simulation cc_compcert_1 (Clight.semantics1 p) (Asm.semantics tp) ->
+  GS.forward_simulation cc_compcert (Clight.semantics1 p) (Asm.semantics tp).
+Proof.
+  intros.
+  unfold cc_compcert, cc_compcert_1 in *.
+Admitted.
+
+Require Import CallConv.
+(*
+Lemma cctrans_ext_compose : cctrans (c_ext @ c_ext) c_ext.
+Proof.
+  constructor.
+  econstructor.
+  - red. intros [mx my Hm] se1 se2 q1 q2 Hse Hq. inv Hse. inv Hq. inv H1. clear Hm1 Hm2.
+    uncklr.
+    exists (se2, (extw m1 m1 (Mem.extends_refl m1), extw m1 m2 Hm)). repeat apply conj; eauto.
+    + econstructor; eauto. constructor. constructor.
+    + exists (cq vf1 sg vargs1 m1). split. econstructor; uncklr; eauto.
+      eapply lessdef_list_refl. constructor.
+      econstructor; uncklr; eauto. constructor.
+    + simpl.
+      Inductive ext_compose_match : ext_world * ext_world -> ext_world -> Prop :=
+      |ext_compose_match_intro m1 m2 Hm11 Hm12,
+        ext_compose_match (extw m1 m2 Hm11, ext2 m1 ) ()
+                                                                            
+        ; 
+Admitted.
+*)
+Lemma cctrans_ro_injp_compose : cctrans ((ro @ c_injp) @ (ro @ c_injp)) (ro @ c_injp).
+Admitted.
+
+Lemma cctrans_ro_wt_c : cctrans (ro @ wt_c) (wt_c @ ro).
+Admitted.
+
+Lemma cctrans_wt_c_ro : cctrans (wt_c @ ro) (ro @ wt_c).
+Admitted.
+
+Lemma cctrans_lessdef_c_ext: cctrans c_ext (lessdef_c @ c_ext).
+Proof.
+  constructor. 
+  econstructor. instantiate (1:= fun a b => a = snd b).
+  - red. intros. destruct w2 as [se [tt [m1 m2 Hm]]].
+    inv H. inv H1. inv H2. destruct H0 as [q' [Hq1 Hq2]].
+    inv Hq1. inv Hq2. inv H7. clear Hm1 Hm2. uncklr.
+    exists (extw m m3 Hm). repeat apply conj.
+    + constructor.
+    + constructor. uncklr. eauto. uncklr.
+      eapply Val.lessdef_list_trans; eauto. constructor. auto.
+    + simpl. reflexivity.
+    + intros r1 r2 [m1' m2' Hm'] wp2 [m1'' m2'' Hm''] Hmat ACE ACI Hr.
+      simpl in ACE, ACI. destruct wp2. inv Hmat. simpl in H0. subst w0.
+      exists (tt, extw m1'' m2'' Hm''). repeat apply conj; simpl; eauto.
+      exists r1. split. destruct r1. econstructor; eauto.
+      eauto.
+  - red. intros [m1 m2 Hm] wp2 [m1' m2' Hm'] se1 se2 q1 q2 Hse Hq ACI Hmat.
+    destruct wp2. simpl in Hmat. subst w0. inv Hse. inv Hq. inv H1. clear Hm1 Hm2.
+    uncklr.
+    exists (se2, (tt, (extw m0 m3 Hm'))). repeat apply conj; simpl; eauto.
+    + exists (cq vf1 sg vargs1 m0). split. econstructor; eauto.
+      eapply lessdef_list_refl.
+      econstructor; uncklr; eauto. constructor.
+    + intros r1 r2 [tt [m1'' m2'' Hm'']]. intros [ACE1 ACE2] [r' [Hr1 Hr2]].
+      simpl in ACE2.
+      exists (extw m1'' m2'' Hm''). repeat apply conj; simpl; eauto.
+      inv Hr1. inv Hr2. inv H7. econstructor; uncklr; eauto.
+      eapply Val.lessdef_trans; eauto. constructor.
+Qed.
+
+Lemma cctrans_wt_c_compose : cctrans (wt_c @ c_injp @ wt_c @ lessdef_c) (wt_c @ c_injp).
+Proof.
+  constructor.
+  econstructor. instantiate (1:= fun a b => fst (snd a) = snd b).
+  - red. intros [se [[se' sg] [j mx my Hm]]] se1 se2 q1 q2 [Hse1 Hse2] [q1' [Hq1 Hq2]]. 
+    inv Hse1. inv Hse2. inv Hq1. inv Hq2. inv H4. clear Hm4 Hm5 Hm6. simpl in H1, H2.
+    simpl in H0. destruct H0. subst sg0. simpl in H. subst se'.
+    (*Compute (GS.ccworld (wt_c @ c_injp @ wt_c @ lessdef_c)).
+     = (Genv.symtbl * (Genv.symtbl * signature * (Genv.symtbl * (injp_world * (Genv.symtbl * (Genv.symtbl * signature * unit))))))%type
+     : Type *)
+    exists (se, (se, sg, (se2, ((injpw j m1 m2 Hm),(se2,(se2,sg,tt)))))). repeat apply conj; simpl; eauto.
+    + repeat apply conj; eauto. constructor; eauto. constructor; eauto.
+    + exists (cq vf1 sg vargs1 m1). split. constructor; eauto.
+      exploit  has_type_inject_list; eauto. intros (vargs2' & Htype & Hinj & Hext).
+      exists (cq vf2 sg vargs2' m2). split. constructor; eauto. constructor.
+      exists (cq vf2 sg vargs2' m2). split. econstructor; eauto.
+      constructor; eauto.
+    +
+      (* Compute (GS.gworld (wt_c @ c_injp @ wt_c @ lessdef_c)). *)
+      intros r1 r2 [t1 [[j' m1' m2' Hm'] [t2 t3]]]. simpl in t1,t2,t3.
+      intros [t4 wp2]. intros [t5 [[j'' m1'' m2'' Hm''] [t6 t7]]].
+      intros Hmatch [_ [ACE [_ _]]] [_ [ACI [_ _]]] Hr.
+      simpl in Hmatch. subst wp2. simpl in ACE, ACI.
+      exists (tt, injpw j'' m1'' m2'' Hm''). repeat apply conj; eauto.
+      rename r2 into r5.
+      destruct Hr as [r2 [Hr1 [r3 [Hr2 [r4 [Hr3 Hr4]]]]]].
+      inv Hr1. inv Hr2. inv H8. clear Hm4 Hm5 Hm6. inv Hr3. inv Hr4. simpl in *.
+      exists (cr vres1 m1'0). split. econstructor; eauto.
+      econstructor; eauto. simpl. eapply Mem.val_inject_lessdef_compose; eauto.
+      constructor.
+  - red.
+    intros [t1 [[j m1 m2 Hm] [t2 t3]]] [t4 wp2].
+    intros [se1 [[se2 sg] [se3 [[j' m1' m2' Hm'] [se4 [[se5 sg'] tt]]]]]].
+    intros se0 se6 q1 q2 Hse1 Hq [_ [ACI [_ _]]] Hr. simpl in ACI.
+    destruct Hse1 as [a [b [c d]]]. inv a. inv b. inv c. inv d. 
+    destruct Hq as [q1' [Hq1 [q2' [Hq2 [q3' [Hq3 Hq4]]]]]].
+    inv Hq1. inv Hq2. inv H5. clear Hm4 Hm5 Hm6. inv Hq3. inv Hq4. simpl in H2, H4.
+    simpl in H0. subst. simpl in H. subst. simpl in Hr. subst wp2. destruct H1. simpl in H. subst.
+    destruct H5. simpl in H. subst. simpl in H0, H1.
+    exists (se1,((se1, sg0), injpw j' m0 m3 Hm')). repeat apply conj; eauto.
+    + simpl. eauto.
+    + split. constructor. reflexivity. constructor; eauto.
+    + simpl.  exists (cq vf1 sg0 vargs1 m0). split. econstructor; eauto.
+      econstructor; eauto. simpl.  
+      eapply val_inject_lessdef_list_compose; eauto. constructor.
+    + intros r1 r2 [t8 [j'' m1'' m2'' Hm'']] [_ ACE] Hr. simpl in ACE.
+      destruct Hr as [r' [Hr1 Hr2]]. inv Hr1. inv Hr2. simpl in H5. inv H9.
+      clear Hm4 Hm5 Hm6. simpl in H.
+      (* Compute (GS.gworld (wt_c @ c_injp @ wt_c @ lessdef_c)). *)
+      exists (tt, ((injpw j'' m1' m2' Hm''), (tt,tt))). repeat apply conj; simpl; eauto.
+      exists (cr vres1 m1'). split. econstructor; eauto.
+      set (res' := Val.ensure_type vres2 (proj_sig_res sg0) ).
+      exists (cr res' m2'). split. econstructor; eauto. simpl.
+      eapply has_type_inject; eauto. constructor.
+      exists (cr res' m2'). split. econstructor; eauto. simpl.
+      eapply Val.ensure_has_type.
+      econstructor; eauto. unfold res'. destruct vres2, (proj_sig_res sg0); auto.
+Qed.
+
+Require Import StackingproofC.
+Lemma cctrans_wt_loc_stacking : cctrans (wt_loc @ cc_stacking_injp) (cc_stacking_injp).
+Proof.
+  constructor. econstructor. instantiate (1:= fun a b => snd a = b).
+  - red. intros [[j m1 my Hm] sg ls1 sp2 m2]. intros.
+    inv H. inv H0. clear Hm4 Hm5 Hm6.
+    Compute GS.ccworld (wt_loc @ cc_stacking injp).
+    exists (se1, (se1, sg, stkw injp (injpw j m1 m2 Hm) sg ls1 sp2 m2)). repeat apply conj; eauto.
+    + econstructor. constructor. constructor. constructor; eauto.
+    + exists (lq vf1 sg ls1 m1). split. econstructor; eauto. constructor.
+      intros l Hl. destruct Hl.
+      * apply always_has_mreg_type.
+      * cbn -[Z.add Z.mul]. rewrite <- (type_of_chunk_of_type ty) at 2.
+        inv H15. destruct H1 as [A B]. exploit B; eauto.
+        intros [b [Hload]]. simpl in H1.
+        eapply (val_has_type_inject); eauto.
+        unfold load_stack in Hload. unfold Mem.loadv in Hload.
+        destr_in Hload.
+        eapply Mem.load_type. eauto.
+      * econstructor; eauto. 
+    + intros r1 r2 [t1 [j' m1' m2' Hm']] wp2 [t2 [j'' m1'' m2'' Hm'']].
+      intros Hmatch [_ ACE] [_ ACI] Hr. simpl in ACE, ACI. simpl in Hmatch. subst wp2.
+      destruct Hr as [r' [Hr1 Hr2]]. inv Hr1. inv Hr2. simpl in H.
+      exists (injpw j'' m1'' m2'' Hm''). repeat apply conj; eauto.
+      econstructor; eauto.
+  - red. intros [t1 [j m1 m2 Hm]] wp2. intros [xse [[xse2 sg] [[j' m1' m2'x Hm'] sg' ls1 sp2 m2']]].
+    intros se1 se2 q1 q2 [Hse1 Hse2] [q' [Hq1 Hq2]] [_ ACI] Hmatch. inv Hse1. inv Hse2. inv Hq1. inv Hq2.
+    simpl in ACI.
+    exists (stkw injp (injpw j' m1' m2' Hm') sg' ls1 sp2 m2'). repeat apply conj; eauto.
+    + econstructor; eauto.
+    + econstructor; eauto.
+    + intros r1 r2 [j'' m1'' m2'' Hm''] ACE Hr. simpl in ACE.
+      exists (tt, injpw j'' m1'' m2'' Hm''). repeat apply conj; simpl; eauto.
+      inv Hr. exists (lr ls1' m1''). split.
+      econstructor. constructor.
+      intros. apply always_has_mreg_type.
+      econstructor; eauto.
+Qed.
+
+Lemma cc_collapse :
+  cctrans
+    ( ro @ c_injp @ 
+      c_injp @
+      (wt_c @ c_ext) @ c_ext @
+      c_injp @
+      c_ext @ c_injp @ c_injp @
+      (ro @ c_injp) @ (ro @ c_injp) @ (ro @ c_injp) @
+      c_injp @                                   (* Unusedglob *)
+      (wt_c @ c_ext @ cc_c_locset) @            (* Alloc *)
+      locset_ext @                              (* Tunneling *)
+      (wt_loc @ cc_stacking_injp) @ (* Stacking *)
+      (mach_ext @ cc_mach_asm)
+    )
+    cc_compcert_1.
+Proof.
+  unfold cc_compcert_1. unfold cc_c_level.
+  etransitivity.
+  
+  rewrite !cc_compose_assoc_2.
+  rewrite (cc_compose_assoc_1 c_injp).
+  rewrite cctrans_injp_comp.
+  
+  rewrite (cc_compose_assoc_1 c_injp).
+  rewrite (cc_compose_assoc_1 (c_injp @ wt_c)).
+  rewrite (cc_compose_assoc_2 c_injp).
+  rewrite move_wt_ext.
+  
+  rewrite !cc_compose_assoc_2.
+  rewrite (cc_compose_assoc_1 c_ext).
+  rewrite  cctrans_ext_comp.
+
+  rewrite (cc_compose_assoc_1 c_injp).
+  rewrite (cc_compose_assoc_1 (c_injp @ c_ext)).
+  rewrite (cc_compose_assoc_2 c_injp).
+  rewrite cctrans_injp_ext.
+
+  rewrite (cc_compose_assoc_1 c_injp).
+  rewrite (cc_compose_assoc_1 (c_injp @ c_ext)).
+  rewrite (cc_compose_assoc_2 c_injp).
+  rewrite cctrans_injp_ext.
+
+  rewrite (cc_compose_assoc_1 c_injp).
+  rewrite cctrans_injp_comp.
+
+  rewrite (cc_compose_assoc_1 ro).
+  rewrite cctrans_ro_wt_c.
+
+  rewrite cc_compose_assoc_2.
+  rewrite !(cc_compose_assoc_1 ro).
+  rewrite (cc_compose_assoc_1 (ro @ c_injp)).
+  rewrite cctrans_ro_injp_compose.
+  rewrite (cc_compose_assoc_1 (ro @ c_injp)).
+  rewrite cctrans_ro_injp_compose.
+  rewrite (cc_compose_assoc_1 (ro @ c_injp)).
+  rewrite cctrans_ro_injp_compose.
+
+  rewrite cc_compose_assoc_2.
+
+  rewrite (cc_compose_assoc_1 c_injp).
+  rewrite cctrans_injp_comp.
+
+  rewrite (cc_compose_assoc_1 wt_c).
+  rewrite cctrans_wt_c_ro.
+
+  rewrite cc_compose_assoc_2.
+  rewrite cctrans_lessdef_c_ext.
+  rewrite cc_compose_assoc_2.
+
+  rewrite (cc_compose_assoc_1 wt_c).
+  rewrite (cc_compose_assoc_1 (wt_c @ _ )).
+  rewrite (cc_compose_assoc_1 ((wt_c @ _ )@_ )).
+  rewrite (cc_compose_assoc_2 (wt_c @ _)).
+  rewrite (cc_compose_assoc_2 wt_c).
+  rewrite cctrans_wt_c_compose.
+
+  rewrite cc_compose_assoc_2.
+  rewrite (cc_compose_assoc_1 wt_loc).
+  rewrite cctrans_wt_loc_stacking.
+
+  rewrite (cc_compose_assoc_1 cc_c_locset).
+  rewrite CL_trans_ext.
+
+  rewrite cc_compose_assoc_2.
+  rewrite (cc_compose_assoc_1 c_ext).
+  rewrite cctrans_ext_comp.
+
+  (*Q1: how to deal with the c_ext*)
+  (*Q2: if we can prove cc_stacking_injp preserving callee_save regs, should we break it into LM? seems
+       we can reuse more results? Or the LM trans lemmas cannot be uses because of the one-wayness?*)
+
+  (** If we can prove Tunneling using injp instead of ext, than we can keep cc_stacking injp as it is*)
+
+Abort.
